Making the bounding lemmas more usable by not requiring to prove that n = n = 1.

theories/OracleBounds.ec
@@ -11,7 +11,12 @@ require import Distr. (* We use core knowledge on probabilities *)
      2) applying the relevant transform,
      3) refactoring to remove the use of Count.
    This is independent of any counting done inside the oracles. *)
-module Count = {
+module type Counter = {
+  fun init(): unit {*}
+  fun incr(): unit
+}.
+
+module Counter = {
   var c:int
 
   fun init(): unit = { c = 0; }
@@ -26,6 +31,52 @@ module type Oracle = {
   fun f(x:from): to
 }.
 
+(* A generic transform to turn any oracle into a counting oracle *)
+module Count (O:Oracle) = {
+  fun f(x:from): to = {
+    var r:to;
+
+    Counter.incr();
+    r = O.f(x);
+    return r;
+  }
+}.
+
+section.
+  declare module O:Oracle {Count}.
+
+  lemma CountO_fL: islossless O.f => islossless Count(O).f.
+  proof strict.
+  by intros=> O_fL; fun;
+     call O_fL;
+     inline Counter.incr; wp.
+  qed.
+
+  lemma CountO_fC ci:
+    islossless O.f =>
+    bd_hoare[Count(O).f: Counter.c = ci ==> Counter.c = ci + 1] = 1%r.
+  proof strict.
+  by intros=> O_fL; fun;
+     call O_fL;
+     inline Counter.incr; wp.
+  qed.
+
+  equiv CountO_fC_E ci:
+    Count(O).f ~ Count(O).f:
+      ={Counter.c, x, glob O} /\ Counter.c{1} = ci ==>
+      ={Counter.c, res, glob O} /\ Counter.c{1} = ci + 1.
+  proof strict.
+  by fun; inline Counter.incr;
+     call (_: true); wp.
+  qed.
+
+  equiv CountO_O: Count(O).f ~ O.f: ={glob O, x} ==> ={glob O, res}.
+  proof strict.
+  by fun*; inline Count(O).f Counter.incr; wp;
+     call (_: true); wp.
+  qed.
+end section.
+
 (* The adversary tries to distinguish between two implementations of f *)
 module type Adv(O:Oracle) = {
   fun distinguish(): bool
@@ -37,7 +88,7 @@ module IND (O:Oracle, A:Adv) = {
   fun main(): bool = {
     var b:bool;
 
-    Count.init();
+    Counter.init();
     b = A.distinguish();
     return b;
   }
@@ -51,11 +102,11 @@ theory Event.
 
   const default:to.
 
-  module Wrap(O:Oracle) = {
+  module Enforce(O:Oracle) = {
     fun f(x:from): to = {
       var r:to = default;
 
-      if (Count.c < bound)
+      if (Counter.c < bound)
         r = O.f(x);
       return r;
     }
@@ -64,79 +115,41 @@ theory Event.
   section.
     declare module O:Oracle {Count}.
     axiom O_fL: islossless O.f.
-    axiom O_fC ci: bd_hoare[O.f: Count.c = ci ==> Count.c = ci + 1] = 1%r.
-    (* We really want to be able to prove this from the previous axiom and the basic equiv knowledge on O.f *)
-    axiom O_fC_E ci: equiv[O.f ~ O.f: ={Count.c, x, glob O} /\ Count.c{1} = ci ==>
-                                      ={Count.c, res, glob O} /\ Count.c{1} = ci + 1].
 
-    declare module A:Adv {O, Count}.
+    declare module A:Adv {Count(O)}.
     axiom A_distinguishL (O <: Oracle {A}):
       islossless O.f =>
       islossless A(O).distinguish.
 
     lemma event_wrap &m:
-      Pr[IND(O,A).main() @ &m: res /\ Count.c <= bound] = Pr[IND(Wrap(O),A).main() @ &m: res].
+      Pr[IND(Count(O),A).main() @ &m: res /\ Counter.c <= bound] <= Pr[IND(Enforce(Count(O)),A).main() @ &m: res].
     proof strict.
-    equiv_deno (_: ={glob A, glob O} ==> Count.c{1} <= bound /\ (Count.c{1} <= bound => ={res}))=> //; last smt.
+    equiv_deno (_: ={glob A, glob O} ==> Counter.c{1} <= bound => res{1} = res{2})=> //; last smt.
     symmetry; fun.
-    call (_: bound < Count.c, ={Count.c, glob O, glob Count}, Count.c{1} <= bound).
+    call (_: !Counter.c <= bound, ={glob Counter, glob O}, Counter.c{1} <= bound).
       (* A lossless *)
       by apply A_distinguishL.
-      (* O.f ~ Wrap(O).f *)
-      fun*; inline Wrap(O).f; case (Count.c{2} = bound).
+      (* Enforce(Count(O)).f ~ Count(O) *)
+      fun*; inline Enforce(Count(O)).f; case (Counter.c{2} = bound).
         rcondf{1} 3; first by progress; wp; skip; smt.
-        exists* Count.c{2}; elim* => c; call{2} (O_fC c).
+        exists* Counter.c{1}; elim* => c; call{2} (CountO_fC O c _); first by apply O_fL.
         by wp; skip; smt.
         rcondt{1} 3; first by progress; wp; skip; smt.
-        wp; exists* Count.c{2}; elim* => c; call (O_fC_E c).
+        wp; exists* Counter.c{2}; elim* => c; call (CountO_fC_E O c).
         by wp; skip; smt.
-      (* Wrap(O).f lossless *)
-      by intros=> _ _; fun; sp; if; first call O_fL.
-      (* O.f preserves bad *)
+      (* Enforce(Count(O)).f lossless *)
+      by progress; fun; sp; if=> //;
+         inline Count(O).f Counter.incr; wp; call O_fL; wp; skip; smt.
+      (* Count(O).f preserves bad *)
       intros=> &m1 //=; bypr; intros=> &m0 bad.
-        cut: 1%r <= Pr[O.f(x{m0}) @ &m0: bound < Count.c]; last smt.
-        cut lbnd: bd_hoare[O.f: Count.c = Count.c{m0} ==> Count.c = Count.c{m0} + 1] >= 1%r;
-          first conseq (O_fC Count.c{m0}).
+        cut: 1%r <= Pr[Count(O).f(x{m0}) @ &m0: bound < Counter.c]; last smt.
+        cut lbnd: bd_hoare[Count(O).f: Counter.c = Counter.c{m0} ==> Counter.c = Counter.c{m0} + 1] >= 1%r;
+          first by conseq (CountO_fC O Counter.c{m0} _); apply O_fL.
         by bdhoare_deno lbnd=> //; smt.
-    call (_: true ==> ={glob Count} /\ Count.c{1} <= bound); first by fun; wp; skip; smt.
-    by skip; smt.
+    by inline Counter.init; wp; skip; smt.
     qed.
   end section.
 end Event.
-
-theory Static.
-  section.
-    (* declare const bound:int. *)
-    const bound:int.
-    axiom leq0_bound: 0 <= bound.
-
-    declare module O:Oracle {Count}.
-    axiom O_fL: islossless O.f.
-    axiom O_fC ci: bd_hoare[O.f: Count.c = ci ==> Count.c = ci + 1] = 1%r.
-    (* We really want to be able to prove this from the previous axiom and the basic equiv knowledge on O.f *)
-    axiom O_fC_E ci: equiv[O.f ~ O.f: ={Count.c, x, glob O} /\ Count.c{1} = ci ==>
-                                      ={Count.c, res, glob O} /\ Count.c{1} = ci + 1].
-
-    declare module A:Adv {O, Count}.
-    axiom A_distinguishL (O <: Oracle {A}):
-      islossless O.f =>
-      islossless A(O).distinguish.
-    axiom AO_distinguishC:
-      bd_hoare[A(O).distinguish: Count.c = 0 ==> Count.c <= bound] = 1%r.
-    axiom AO_distinguishC_E:
-      equiv[A(O).distinguish ~ A(O).distinguish:
-        ={Count.c, glob O, glob A} /\ Count.c{1} = 0 ==>
-        ={Count.c, glob O, glob A, res} /\ Count.c{1} <= bound].
-
-    lemma bndAdv_event &m:
-      Pr[IND(O,A).main() @ &m: res] = Pr[IND(O,A).main() @ &m: res /\ Count.c <= bound].
-    proof strict.
-    equiv_deno (_: ={glob A, glob O} ==> ={Count.c, res} /\ Count.c{1} <= bound)=> //; fun.
-    call AO_distinguishC_E.
-    by call (_: true ==> ={Count.c} /\ Count.c{1} = 0); first by fun; wp.
-    qed.
-  end section.
-end Static.
 
 (** Ideally, this theory would allow transitions between penalty-style
     bounds on the number of oracle queries and cryptographer-friendly
@@ -153,7 +166,7 @@ theory StaticWrap.
     fun f(x:from): to = {
       var r:to = default;
 
-      if (Count.c < bound)
+      if (Counter.c < bound)
         r = O.f(x);
       return r;
     }
@@ -164,50 +177,48 @@ theory StaticWrap.
   section.
     declare module O:Oracle {Count}.
     axiom O_fL: islossless O.f.
-    axiom O_fC ci: bd_hoare[O.f: Count.c = ci ==> Count.c = ci + 1] = 1%r.
-    (* We really want to be able to prove this from the previous axiom and the basic equiv knowledge on O.f *)
-    axiom O_fC_E ci: equiv[O.f ~ O.f: ={Count.c, x, glob O} /\ Count.c{1} = ci ==>
-                                      ={Count.c, res, glob O} /\ Count.c{1} = ci + 1].
 
-    declare module A:Adv {O, Count}.
+    declare module A:Adv {Count(O)}.
     axiom A_distinguishL (O <: Oracle {A}):
       islossless O.f =>
       islossless A(O).distinguish.
 
     lemma wrapAdv_bnd:
-      bd_hoare[WrapAdv(A,O).distinguish: Count.c = 0 ==> Count.c <= bound] = 1%r.
+      bd_hoare[WrapAdv(A,Count(O)).distinguish: Counter.c = 0 ==> Counter.c <= bound] = 1%r.
     proof strict.
-      fun (Count.c <= bound)=> //; first by smt.
+      fun (Counter.c <= bound)=> //; first by smt.
         by apply A_distinguishL.
-      by fun; sp; if; [exists* Count.c; elim* => c; call (O_fC c) |].
+      by fun; sp; if;
+           [exists* Counter.c; elim* => c; call (CountO_fC O c _); first apply O_fL |];
+         skip; smt.
     qed.
 
     lemma event_bndAdv &m:
-      Pr[IND(O,A).main() @ &m: res /\ Count.c <= bound] = Pr[IND(O,WrapAdv(A)).main() @ &m: res].
+      Pr[IND(Count(O),A).main() @ &m: res /\ Counter.c <= bound] <= Pr[IND(Count(O),WrapAdv(A)).main() @ &m: res].
     proof strict.
-    equiv_deno (_: ={glob A, glob O} ==> ={res, glob Count} /\ Count.c{1} <= bound)=> //.
+    equiv_deno (_: ={glob A, glob O} ==> Counter.c{1} <= bound => ={res, glob Count})=> //; last smt.
     symmetry; fun.
-    call (_: bound < Count.c, ={glob Count, glob Wrap, glob O}).
+    call (_: bound < Counter.c, ={glob Counter, glob Wrap, glob O}).
       (* A lossless *)
       by apply A_distinguishL.
       (* Wrap(O).f ~ O.f *)
-      fun*; inline Wrap(O).f; case (Count.c{1} = bound).
+      fun*; inline Wrap(Count(O)).f; case (Counter.c{1} = bound).
         rcondf{1} 3; first by progress; wp.
-        exists* Count.c{2}; elim* => c; call{2} (O_fC c).
+        exists* Counter.c{2}; elim* => c; call{2} (CountO_fC O c _);
+          first apply O_fL.
         by wp; skip; smt.
         rcondt{1} 3; first by progress; wp; skip; smt.
-        wp; exists* Count.c{2}; elim* => c; call (O_fC_E c).
+        wp; exists* Counter.c{2}; elim* => c; call (CountO_fC_E O c).
         by wp.
       (* Wrap(O).f lossless *)
-      by progress; fun; sp; if; [call (O_fL) |].
+      by progress; fun; sp; if; [call (CountO_fL O _); first apply O_fL |].
       (* O.f preserves bad *)
       progress; bypr; intros=> &m0 bad.
-      cut: 1%r <= Pr[O.f(x{m0}) @ &m0: bound < Count.c]; last smt.
-      cut lbnd: bd_hoare[O.f: Count.c = Count.c{m0} ==> Count.c = Count.c{m0} + 1] >= 1%r;
-        first by conseq (O_fC Count.c{m0}).
+      cut: 1%r <= Pr[Count(O).f(x{m0}) @ &m0: bound < Counter.c]; last smt.
+      cut lbnd: bd_hoare[Count(O).f: Counter.c = Counter.c{m0} ==> Counter.c = Counter.c{m0} + 1] >= 1%r;
+        first by conseq (CountO_fC O Counter.c{m0} _); first apply O_fL.
       by bdhoare_deno lbnd; last smt.
-    call (_: true ==> ={glob Count} /\ Count.c{1} = 0);
-      first by fun; wp.
+    inline Counter.init; wp.
     by skip; smt.
     qed.
   end section.
